theories/Substitution/Conversion.v
@@ -1,6 +1,7 @@
 From LogRel.AutoSubst Require Import core unscoped Ast Extra.
 From LogRel Require Import Utils BasicAst Notations Context NormalForms Weakening GenericTyping LogicalRelation Validity.
 From LogRel.LogicalRelation Require Import Irrelevance Escape Reflexivity Weakening Neutral.
+From LogRel.Substitution Require Import Properties Irrelevance.
 
 Set Universe Polymorphism.
 
@@ -46,5 +47,277 @@ Proof.
   1: now unshelve now eapply validTyEq.
   now eapply validTmEq.
 Qed.
+
+
+Lemma convSubstCtx1 {Γ Δ A B l σ} 
+  (VΓ : [||-v Γ])
+  (wfΔ : [|- Δ])
+  (VΓA : [||-v Γ ,, A]) 
+  (VΓB : [||-v Γ ,, B]) 
+  (VA : [_ ||-v<l> A | VΓ])
+  (VB : [_ ||-v<l> B | VΓ])
+  (VAB : [_ ||-v<l> A ≅ B | VΓ | VA])
+  (Vσ : [_ ||-v σ : _ | VΓA | wfΔ]) :
+  [_ ||-v σ : _ | VΓB | wfΔ].
+Proof.
+  pose proof (invValiditySnoc VΓA) as [? [? [?]]]; subst.
+  pose proof (invValiditySnoc VΓB) as [? [? [?]]]; subst.
+  eapply irrelevanceSubstExt.
+  1: rewrite <- scons_eta'; reflexivity.
+  unshelve eapply consSubstS.
+  1: epose (validTail Vσ); irrValid.
+  eapply LRTmRedConv.
+  2: irrelevanceRefl; eapply validHead.
+  now eapply validTyEq.
+  Unshelve. 6: tea.
+    2: eapply irrelevanceSubst; now eapply validTail.
+    tea.
+Qed.
+
+Lemma convSubstEqCtx1 {Γ Δ A B l σ σ'} 
+  (VΓ : [||-v Γ])
+  (wfΔ : [|- Δ])
+  (VΓA : [||-v Γ ,, A]) 
+  (VΓB : [||-v Γ ,, B]) 
+  (VA : [_ ||-v<l> A | VΓ])
+  (VB : [_ ||-v<l> B | VΓ])
+  (VAB : [_ ||-v<l> A ≅ B | VΓ | VA])
+  (Vσ : [_ ||-v σ : _ | VΓA | wfΔ]) 
+  (Vσ' : [_ ||-v σ' : _ | VΓA | wfΔ]) 
+  (Vσσ' : [_ ||-v σ ≅ σ' : _ | VΓA | wfΔ | Vσ]) 
+  (VσB : [_ ||-v σ : _ | VΓB | wfΔ]) :
+  [_ ||-v σ ≅ σ' : _ | VΓB | wfΔ | VσB].
+Proof.
+  pose proof (invValiditySnoc VΓA) as [? [? [?]]]; subst.
+  pose proof (invValiditySnoc VΓB) as [? [? [?]]]; subst.
+  eapply irrelevanceSubstEq.
+  eapply irrelevanceSubstEqExt.
+  1: rewrite <- scons_eta'; reflexivity.
+  unshelve eapply consSubstSEq'.
+  8: now eapply eqTail.
+  3: irrValid.
+  3: eapply LRTmEqRedConv.
+  4: now eapply eqHead.
+  2: irrelevanceRefl; eapply validTyEq; irrValid.
+  eapply LRTmRedConv.
+  2: irrelevanceRefl; eapply validHead.
+  eapply validTyExt.
+  1: now eapply validTail.
+  eapply reflSubst.
+  Unshelve.
+  1: now rewrite scons_eta'.
+  9: tea.
+  7: tea.
+  2,6: irrValid.
+  1,2: tea.
+  1,2: eapply irrelevanceSubst; now eapply validTail.
+Qed.
+
+
+Lemma convCtx1 {Γ A B P l} 
+  (VΓ : [||-v Γ])
+  (VΓA : [||-v Γ ,, A]) 
+  (VΓB : [||-v Γ ,, B]) 
+  (VA : [_ ||-v<l> A | VΓ])
+  (VB : [_ ||-v<l> B | VΓ])
+  (VAB : [_ ||-v<l> A ≅ B | VΓ | VA])
+  (VP : [_ ||-v<l> P | VΓA]) :
+  [_ ||-v<l> P | VΓB].
+Proof.
+  opector; intros.
+  - eapply validTy; tea; eapply convSubstCtx1; tea; now eapply symValidEq.
+  - irrelevanceRefl; unshelve eapply validTyExt.
+    3,4: tea. 
+    1,2:  eapply convSubstCtx1; tea; now eapply symValidEq.
+    eapply convSubstEqCtx1; cycle 2; tea; now eapply symValidEq.
+    Unshelve. all: tea.
+Qed.
+
+Lemma convEqCtx1 {Γ A B P Q l} 
+  (VΓ : [||-v Γ])
+  (VΓA : [||-v Γ ,, A]) 
+  (VΓB : [||-v Γ ,, B]) 
+  (VA : [_ ||-v<l> A | VΓ])
+  (VB : [_ ||-v<l> B | VΓ])
+  (VAB : [_ ||-v<l> A ≅ B | VΓ | VA])
+  (VP : [_ ||-v<l> P | VΓA])
+  (VPB : [_ ||-v<l> P | VΓB])
+  (VPQ : [_ ||-v<l> P ≅ Q | VΓA | VP]) :
+  [_ ||-v<l> P ≅ Q | VΓB | VPB].
+Proof.
+  constructor; intros; irrelevanceRefl.
+  eapply validTyEq; tea.
+  Unshelve. 1: tea. 
+  unshelve eapply convSubstCtx1; cycle 5; tea; now eapply symValidEq.
+Qed.
+
+Lemma convSubstCtx2 {Γ Δ A1 B1 A2 B2 l σ} 
+  (VΓ : [||-v Γ])
+  (wfΔ : [|- Δ])
+  (VA1 : [_ ||-v<l> A1 | VΓ])
+  (VB1 : [_ ||-v<l> B1 | VΓ])
+  (VAB1 : [_ ||-v<l> A1 ≅ B1 | VΓ | VA1])
+  (VΓA1 := validSnoc VΓ VA1) 
+  (VΓB1 := validSnoc VΓ VB1) 
+  (VA2 : [_ ||-v<l> A2 | VΓA1])
+  (VB2 : [_ ||-v<l> B2 | VΓA1])
+  (VAB : [_ ||-v<l> A2 ≅ B2 | VΓA1 | VA2])
+  (VB2' := convCtx1 VΓ VΓA1 VΓB1 VA1 VB1 VAB1 VB2)
+  (VΓA12 := validSnoc VΓA1 VA2) 
+  (VΓB12 := validSnoc VΓB1 VB2') 
+  (Vσ : [_ ||-v σ : _ | VΓA12 | wfΔ]) :
+  [_ ||-v σ : _ | VΓB12 | wfΔ].
+Proof.
+  eapply irrelevanceSubstExt.
+  1: rewrite <- scons_eta'; reflexivity.
+  unshelve eapply consSubstS.
+  + eapply convSubstCtx1; tea.
+    now eapply validTail.
+  + eapply LRTmRedConv.
+    2: now eapply validHead.
+    eapply validTyEq; tea.
+  Unshelve. all: tea.
+Qed.
+
+Lemma convSubstCtx2' {Γ Δ A1 B1 A2 B2 l σ} 
+  (VΓ : [||-v Γ])
+  (wfΔ : [|- Δ])
+  (VΓA1 : [||-v Γ ,, A1]) 
+  (VΓA12 : [||-v Γ ,, A1 ,, A2]) 
+  (VΓB12 : [||-v Γ ,, B1 ,, B2]) 
+  (VA1 : [_ ||-v<l> A1 | VΓ])
+  (VB1 : [_ ||-v<l> B1 | VΓ])
+  (VAB1 : [_ ||-v<l> A1 ≅ B1 | VΓ | VA1])
+  (VA2 : [_ ||-v<l> A2 | VΓA1])
+  (VB2 : [_ ||-v<l> B2 | VΓA1])
+  (VAB : [_ ||-v<l> A2 ≅ B2 | VΓA1 | VA2])
+  (Vσ : [_ ||-v σ : _ | VΓA12 | wfΔ]) :
+  [_ ||-v σ : _ | VΓB12 | wfΔ].
+Proof.
+  eapply irrelevanceSubst.
+  eapply convSubstCtx2; irrValid.
+  Unshelve. all: tea; irrValid.
+Qed.
+
+Lemma convSubstEqCtx2 {Γ Δ A1 B1 A2 B2 l σ σ'} 
+  (VΓ : [||-v Γ])
+  (wfΔ : [|- Δ])
+  (VA1 : [_ ||-v<l> A1 | VΓ])
+  (VB1 : [_ ||-v<l> B1 | VΓ])
+  (VAB1 : [_ ||-v<l> A1 ≅ B1 | VΓ | VA1])
+  (VΓA1 := validSnoc VΓ VA1) 
+  (VΓB1 := validSnoc VΓ VB1) 
+  (VA2 : [_ ||-v<l> A2 | VΓA1])
+  (VB2 : [_ ||-v<l> B2 | VΓA1])
+  (VAB : [_ ||-v<l> A2 ≅ B2 | VΓA1 | VA2])
+  (VB2' := convCtx1 VΓ VΓA1 VΓB1 VA1 VB1 VAB1 VB2)
+  (VΓA12 := validSnoc VΓA1 VA2) 
+  (VΓB12 := validSnoc VΓB1 VB2') 
+  (Vσ : [_ ||-v σ : _ | VΓA12 | wfΔ]) 
+  (Vσ' : [_ ||-v σ' : _ | VΓA12 | wfΔ]) 
+  (Vσσ' : [_ ||-v σ ≅ σ' : _ | VΓA12 | wfΔ | Vσ]) 
+  (VσB : [_ ||-v σ : _ | VΓB12 | wfΔ]) :
+  [_ ||-v σ ≅ σ' : _ | VΓB12 | wfΔ | VσB].
+Proof.
+  eapply irrelevanceSubstEq.
+  eapply irrelevanceSubstEqExt.
+  1: rewrite <- scons_eta'; reflexivity.
+  unshelve eapply consSubstSEq'.
+  8:{ eapply convSubstEqCtx1; tea.
+    1: now eapply validTail.
+    now eapply eqTail.
+  }
+  3,4: irrValid.
+  2: eapply convSubstCtx1; tea; now eapply validTail. 
+  3: eapply LRTmEqRedConv.
+  4: now eapply eqHead.
+  2: irrelevanceRefl; eapply validTyEq; irrValid.
+  eapply LRTmRedConv.
+  2: irrelevanceRefl; eapply validHead.
+  eapply validTyExt.
+  1: now eapply validTail.
+  eapply reflSubst.
+  Unshelve.
+  1: now rewrite scons_eta'.
+  11: tea.
+  1,2,6: irrValid.
+  1: tea.
+  2: eapply convSubstCtx1; tea.
+  1,2: now eapply validTail.
+Qed. 
+
+Lemma convSubstEqCtx2' {Γ Δ A1 B1 A2 B2 l σ σ'} 
+  (VΓ : [||-v Γ])
+  (wfΔ : [|- Δ])
+  (VA1 : [_ ||-v<l> A1 | VΓ])
+  (VB1 : [_ ||-v<l> B1 | VΓ])
+  (VAB1 : [_ ||-v<l> A1 ≅ B1 | VΓ | VA1])
+  (VΓA1 : [||-v Γ ,, A1]) 
+  (VΓB1 : [||-v Γ ,, B1]) 
+  (VA2 : [_ ||-v<l> A2 | VΓA1])
+  (VB2 : [_ ||-v<l> B2 | VΓA1])
+  (VAB : [_ ||-v<l> A2 ≅ B2 | VΓA1 | VA2])
+  (VB2' : [_ ||-v<l> B2 | VΓB1])
+  (VΓA12 : [||-v Γ ,, A1 ,, A2]) 
+  (VΓB12 : [||-v Γ ,, B1,, B2]) 
+  (Vσ : [_ ||-v σ : _ | VΓA12 | wfΔ]) 
+  (Vσ' : [_ ||-v σ' : _ | VΓA12 | wfΔ]) 
+  (Vσσ' : [_ ||-v σ ≅ σ' : _ | VΓA12 | wfΔ | Vσ]) 
+  (VσB : [_ ||-v σ : _ | VΓB12 | wfΔ]) :
+  [_ ||-v σ ≅ σ' : _ | VΓB12 | wfΔ | VσB].
+Proof.
+  eapply irrelevanceSubstEq.
+  eapply convSubstEqCtx2; irrValid.
+  Unshelve.  all: tea; irrValid.
+Qed.
+
+Lemma convCtx2 {Γ A1 B1 A2 B2 P l} 
+  (VΓ : [||-v Γ])
+  (VA1 : [_ ||-v<l> A1 | VΓ])
+  (VB1 : [_ ||-v<l> B1 | VΓ])
+  (VAB1 : [_ ||-v<l> A1 ≅ B1 | VΓ | VA1])
+  (VΓA1 := validSnoc VΓ VA1) 
+  (VΓB1 := validSnoc VΓ VB1) 
+  (VA2 : [_ ||-v<l> A2 | VΓA1])
+  (VB2 : [_ ||-v<l> B2 | VΓA1])
+  (VAB : [_ ||-v<l> A2 ≅ B2 | VΓA1 | VA2])
+  (VB2' := convCtx1 VΓ VΓA1 VΓB1 VA1 VB1 VAB1 VB2)
+  (VΓA12 := validSnoc VΓA1 VA2) 
+  (VΓB12 := validSnoc VΓB1 VB2') 
+  (VP : [_ ||-v<l> P | VΓA12]) :
+  [_ ||-v<l> P | VΓB12].
+Proof.
+  assert [_ ||-v<l> A2 | VΓB1] by now eapply convCtx1.
+  assert [_ ||-v<l> B1 ≅ A1 | _ | VB1] by now eapply symValidEq.
+  assert [_ ||-v<l> B2 ≅ A2 | _ | VB2'] by (eapply convEqCtx1; tea; now eapply symValidEq).
+  opector; intros.
+  - eapply validTy; tea; now eapply convSubstCtx2'.
+  - irrelevanceRefl; unshelve eapply validTyExt.
+    3,4: tea. 
+    1,2:  now eapply convSubstCtx2'.
+    eapply convSubstEqCtx2'; tea.
+    Unshelve. tea.
+Qed.
+
+Lemma convCtx2' {Γ A1 A2 B1 B2 P l} 
+  (VΓ : [||-v Γ])
+  (VA1 : [_ ||-v<l> A1 | VΓ])
+  (VB1 : [_ ||-v<l> B1 | VΓ])
+  (VAB1 : [_ ||-v<l> A1 ≅ B1 | VΓ | VA1])
+  (VΓA1 : [||-v Γ ,, A1]) 
+  (VΓB1 : [||-v Γ ,, B1]) 
+  (VA2 : [_ ||-v<l> A2 | VΓA1])
+  (VB2 : [_ ||-v<l> B2 | VΓA1])
+  (VAB : [_ ||-v<l> A2 ≅ B2 | VΓA1 | VA2])
+  (VB2' : [_ ||-v<l> B2 | VΓB1])
+  (VΓA12 : [||-v Γ ,, A1 ,, A2]) 
+  (VΓB12 : [||-v Γ ,, B1,, B2])
+  (VP : [_ ||-v<l> P | VΓA12]) :
+  [_ ||-v<l> P | VΓB12].
+Proof.
+  eapply irrelevanceValidity; eapply convCtx2; irrValid.
+  Unshelve. all: tea; irrValid.
+Qed.
+
 
 End Conversion.
