theories/Substitution/Introductions/Poly.v
@@ -146,12 +146,12 @@ Section PolyValidity.
     : PolyRedEq PABt A B[u]⇑.
   Proof.
     constructor.
-    - intros; eapply LRTyEqRefl_.
+    - intros; eapply reflLRTyEq.
     - intros; irrelevance0; rewrite liftSubst_scons_eq; [reflexivity|].
       unshelve eapply PolyRed.posExt; cycle 1; tea.
       + eapply Rt; now irrelevanceRefl.
       + eapply Ru; now irrelevanceRefl.
-      + eapply Rtu; try eapply LREqTermRefl_; now irrelevanceRefl.
+      + eapply Rtu; try eapply reflLRTmEq; now irrelevanceRefl.
   Qed.
   
   Context {l Γ F G} (VΓ : [||-v Γ])
